Reduce time complexity of type checking with Factory, prove termination of LExpr.resolveAux
This patch

- Avoids recursive traversal of body of LFuncs in Factory during type checking. Instead, the bodys are typechecked separately.
- Proves termination of LExpr.resolveAux. The above refactoring enabled this :)
- And adds tiny well-formedness statements about type variables of LFunc.

Strata/DL/Lambda/Factory.lean
@@ -84,6 +84,7 @@ an example of a `concreteEval` function for `Int.Add`:
 
 Note that if there is an arity mismatch or if the arguments are not
 concrete/constants, this fails and it returns .none.
+If LFunc already has body, it must not have concreteEval, and vice versa.
 
 (TODO) Use `.bvar`s in the body to correspond to the formals instead of using
 `.fvar`s.
@@ -102,36 +103,6 @@ structure LFunc (T : LExprParams) where
   -- resulting expression of concreteEval if evaluation was successful.
   concreteEval : Option (T.Metadata → List (LExpr T.mono) → Option (LExpr T.mono)) := .none
   axioms   : List (LExpr T.mono) := []  -- For axiomatic definitions
-
-/--
-Well-formedness properties of LFunc. These are split from LFunc because
-otherwise it becomes impossible to create a 'temporary' LFunc object whose
-wellformedness might not hold yet.
--/
-structure LFuncWF {T : LExprParams} (f : LFunc T) where
-  -- No args have same name.
-  arg_nodup:
-    List.Nodup (f.inputs.map (·.1.name))
-  -- Free variables of body must be arguments.
-  body_freevars:
-    ∀ b, f.body = .some b →
-      (LExpr.freeVars b).map (·.1.name) ⊆ f.inputs.map (·.1.name)
-  -- concreteEval does not succeed if the length of args is incorrect.
-  concreteEval_argmatch:
-    ∀ fn md args res, f.concreteEval = .some fn
-      → fn md args = .some res
-      → args.length = f.inputs.length
-
-instance LFuncWF.arg_nodup_decidable {T : LExprParams} (f : LFunc T):
-    Decidable (List.Nodup (f.inputs.map (·.1.name))) := by
-  apply List.nodupDecidable
-
-instance LFuncWF.body_freevars_decidable {T : LExprParams} (f : LFunc T):
-    Decidable (∀ b, f.body = .some b →
-      (LExpr.freeVars b).map (·.1.name) ⊆ f.inputs.map (·.1.name)) :=
-  by exact f.body.decidableForallMem
-
--- LFuncWF.concreteEval_argmatch is not decidable.
 
 instance [Inhabited T.Metadata] [Inhabited T.IDMeta] : Inhabited (LFunc T) where
   default := { name := Inhabited.default, inputs := [], output := LMonoTy.bool }
@@ -182,7 +153,7 @@ def LFunc.outputPolyType (f : (LFunc T)) : LTy :=
 
 def LFunc.eraseTypes (f : LFunc T) : LFunc T :=
   { f with
-    body := f.body.map LExpr.eraseTypes,
+    body := f.body.map LExpr.eraseTypes
     axioms := f.axioms.map LExpr.eraseTypes
   }
 
@@ -205,19 +176,6 @@ instance : Inhabited (@Factory T) where
 instance : Membership (LFunc T) (@Factory T) where
   mem x f := Array.Mem x f
 
-/--
-Well-formedness properties of Factory.
--/
-structure FactoryWF {T : LExprParams} (fac:Factory T) where
-  name_nodup:
-    List.Nodup (fac.toList.map (·.name.name))
-  lfuncs_wf:
-    ∀ (lf:LFunc T), lf ∈ fac → LFuncWF lf
-
-instance FactoryWF.name_nodup_decidable {T : LExprParams} (fac : Factory T):
-    Decidable (List.Nodup (fac.toList.map (·.name.name))) := by
-  apply List.nodupDecidable
-
 
 def Factory.getFunctionNames (F : @Factory T) : Array T.Identifier :=
   F.map (fun f => f.name)
@@ -239,88 +197,11 @@ def Factory.addFactoryFunc (F : @Factory T) (func : LFunc T) : Except Diagnostic
 
 
 /--
-If Factory.addFactoryFunc succeeds, and the input factory & LFunc were already
-well-formed, the returned factory is also well-formed.
--/
-theorem Factory.addFactoryFunc_wf
-  (F : @Factory T) (F_wf: FactoryWF F) (func : LFunc T) (func_wf: LFuncWF func):
-  ∀ F', F.addFactoryFunc func = .ok F' → FactoryWF F' :=
-by
-  unfold Factory.addFactoryFunc
-  unfold Factory.getFactoryLFunc
-  intros F' Hmatch
-  split at Hmatch -- Case-analysis on the match condition
-  · rename_i heq
-    cases Hmatch -- F' is Array.push F
-    apply FactoryWF.mk
-    · have Hnn := F_wf.name_nodup
-      grind [Array.toList_push,List]
-    · intros lf Hmem
-      rw [Array.mem_push] at Hmem
-      cases Hmem
-      · have Hwf := F_wf.lfuncs_wf
-        apply Hwf; assumption
-      · grind
-  · grind
-
-/--
 Append a factory `newF` to an existing factory `F`, checking for redefinitions
 along the way.
 -/
 def Factory.addFactory (F newF : @Factory T) : Except DiagnosticModel (@Factory T) :=
   Array.foldlM (fun factory func => factory.addFactoryFunc func) F newF
-
-
-/--
-If Factory.addFactory succeeds, and the input two factories were already
-well-formed, the returned factory is also well-formed.
--/
-theorem Factory.addFactory_wf
-  (F : @Factory T) (F_wf: FactoryWF F) (newF : @Factory T)
-  (newF_wf: FactoryWF newF):
-  ∀ F', F.addFactory newF = .ok F' → FactoryWF F' :=
-by
-  unfold Factory.addFactory
-  rw [← Array.foldlM_toList]
-  generalize Hl: newF.toList = l
-  induction l generalizing newF F
-  · rw [Array.toList_eq_nil_iff] at Hl
-    rw [List.foldlM_nil]
-    unfold Pure.pure Except.instMonad Except.pure
-    grind
-  · rename_i lf lf_tail tail_ih
-    have Hl: newF = (List.toArray [lf]) ++ (List.toArray lf_tail) := by grind
-    have Htail_wf: FactoryWF (lf_tail.toArray) := by
-      rw [Hl] at newF_wf
-      apply FactoryWF.mk
-      · have newF_wf_name_nodup := newF_wf.name_nodup
-        grind
-      · intro lf
-        have newF_wf_lfuncs_wf := newF_wf.lfuncs_wf lf
-        intro Hmem
-        apply newF_wf_lfuncs_wf
-        apply Array.mem_append_right
-        assumption
-    have Hhead_wf: LFuncWF lf := by
-      rw [Hl] at newF_wf
-      have Hwf := newF_wf.lfuncs_wf
-      apply Hwf
-      apply Array.mem_append_left
-      grind
-    intro F'
-    simp only [List.foldlM]
-    unfold bind
-    unfold Except.instMonad
-    simp only []
-    unfold Except.bind
-    intro H
-    split at H
-    · contradiction
-    · rename_i F_interm HaddFacFun
-      have HF_interm_wf: FactoryWF F_interm := by
-        apply (Factory.addFactoryFunc_wf F F_wf lf) <;> assumption
-      simp only [] at H
-      apply tail_ih F_interm HF_interm_wf (lf_tail.toArray) <;> grind
 
 
 def getLFuncCall {GenericTy} (e : LExpr ⟨T, GenericTy⟩) : LExpr ⟨T, GenericTy⟩ × List (LExpr ⟨T, GenericTy⟩) :=
