Strata/DL/Lambda/FactoryWF.lean
@@ -1,0 +1,187 @@
+/-
+  Copyright Strata Contributors
+
+  SPDX-License-Identifier: Apache-2.0 OR MIT
+-/
+
+import Strata.DL.Lambda.Factory
+import Strata.DL.Lambda.LExprEval
+import Strata.DL.Lambda.LExprWF
+import Strata.DL.Lambda.LTy
+import Strata.DL.Lambda.LExprTypeSpec
+import Strata.DL.Lambda.Semantics
+import Strata.DDM.Util.Array
+import Strata.DL.Util.List
+import Strata.DL.Util.ListMap
+
+/-!
+## Well-formedness of LFunc and Factory
+-/
+
+namespace Lambda
+
+open Std (ToFormat Format format)
+
+variable {T : LExprParams} [Inhabited T.Metadata] [ToFormat T.IDMeta]
+
+/--
+Well-formedness properties of LFunc. These are split from LFunc because
+otherwise it becomes impossible to create a 'temporary' LFunc object whose
+wellformedness might not hold yet.
+-/
+structure LFuncWF (f : LFunc T) where
+  -- No args have same name.
+  arg_nodup:
+    List.Nodup (f.inputs.map (·.1.name))
+  -- Free variables of body must be arguments.
+  body_freevars:
+    ∀ b, f.body = .some b →
+      (LExpr.freeVars b).map (·.1.name) ⊆ f.inputs.map (·.1.name)
+  -- concreteEval does not succeed if the length of args is incorrect.
+  concreteEval_argmatch:
+    ∀ fn md args res, f.concreteEval = .some fn
+      → fn md args = .some res
+      → args.length = f.inputs.length
+  -- body and concreteEval cannot exist at once
+  body_or_concreteEval:
+    ¬ (f.concreteEval.isSome ∧ f.body.isSome)
+  -- No typeArgs have same name
+  typeArgs_nodup:
+    List.Nodup f.typeArgs
+  -- All type vars in input and output are in typeArg
+  inputs_typevars_in_typeArgs:
+    ∀ ty, ty ∈ f.inputs.values →
+      ty.freeVars ⊆ f.typeArgs
+  output_typevars_in_typeArgs:
+    f.output.freeVars ⊆ f.typeArgs
+
+
+instance LFuncWF.arg_nodup_decidable {T : LExprParams} (f : LFunc T):
+    Decidable (List.Nodup (f.inputs.map (·.1.name))) := by
+  apply List.nodupDecidable
+
+instance LFuncWF.body_freevars_decidable {T : LExprParams} (f : LFunc T):
+    Decidable (∀ b, f.body = .some b →
+      (LExpr.freeVars b).map (·.1.name) ⊆ f.inputs.map (·.1.name)) :=
+  by exact f.body.decidableForallMem
+
+-- LFuncWF.concreteEval_argmatch is not decidable.
+
+instance LFuncWF.body_or_concreteEval_decidable (f : LFunc T):
+    Decidable (¬ (f.concreteEval.isSome ∧ f.body.isSome)) :=
+  if H:f.concreteEval.isSome && f.body.isSome then by
+    apply isFalse; grind
+  else by apply isTrue; grind
+
+instance LFuncWF.typeArgs_decidable (f : LFunc T):
+    Decidable (List.Nodup f.typeArgs) := by
+  apply List.nodupDecidable
+
+instance LFuncWF.inputs_typevars_in_typeArgs_decidable {f : LFunc T}:
+    Decidable (∀ ty, ty ∈ f.inputs.values →
+      ty.freeVars ⊆ f.typeArgs) :=
+  if Hall:f.inputs.values.all (fun ty => ty.freeVars ⊆ f.typeArgs)
+  then by
+    apply isTrue; grind
+  else by
+    apply isFalse; grind
+
+instance LFuncWF.output_typevars_in_typeArgs_decidable {f : LFunc T}:
+    Decidable (f.output.freeVars ⊆ f.typeArgs) :=
+  if Hall: f.output.freeVars ⊆ f.typeArgs then by apply isTrue; grind
+  else by apply isFalse; grind
+
+
+/--
+Well-formedness properties of Factory.
+-/
+structure FactoryWF (fac:Factory T) where
+  name_nodup:
+    List.Nodup (fac.toList.map (·.name.name))
+  lfuncs_wf:
+    ∀ (lf:LFunc T), lf ∈ fac → LFuncWF lf
+
+
+instance FactoryWF.name_nodup_decidable (fac : Factory T):
+    Decidable (List.Nodup (fac.toList.map (·.name.name))) := by
+  apply List.nodupDecidable
+
+/--
+If Factory.addFactoryFunc succeeds, and the input factory & LFunc were already
+well-formed, the returned factory is also well-formed.
+-/
+theorem Factory.addFactoryFunc_wf
+  (F : @Factory T) (F_wf: FactoryWF F) (func : LFunc T) (func_wf: LFuncWF func):
+  ∀ F', F.addFactoryFunc func = .ok F' → FactoryWF F' :=
+by
+  unfold Factory.addFactoryFunc
+  unfold Factory.getFactoryLFunc
+  intros F' Hmatch
+  split at Hmatch <;> try grind -- Case-analysis on the match condition
+  rename_i heq
+  cases Hmatch -- F' is Array.push F
+  apply FactoryWF.mk
+  case name_nodup =>
+    have Hnn := F_wf.name_nodup
+    grind [Array.toList_push,List]
+  case lfuncs_wf =>
+    intros lf Hmem
+    rw [Array.mem_push] at Hmem
+    cases Hmem
+    · have Hwf := F_wf.lfuncs_wf
+      apply Hwf; assumption
+    · grind
+
+
+/--
+If Factory.addFactory succeeds, and the input two factories were already
+well-formed, the returned factory is also well-formed.
+-/
+theorem Factory.addFactory_wf
+  (F : @Factory T) (F_wf: FactoryWF F) (newF : @Factory T)
+  (newF_wf: FactoryWF newF):
+  ∀ F', F.addFactory newF = .ok F' → FactoryWF F' :=
+by
+  unfold Factory.addFactory
+  rw [← Array.foldlM_toList]
+  generalize Hl: newF.toList = l
+  induction l generalizing newF F
+  · rw [Array.toList_eq_nil_iff] at Hl
+    rw [List.foldlM_nil]
+    unfold Pure.pure Except.instMonad Except.pure
+    grind
+  · rename_i lf lf_tail tail_ih
+    have Hl: newF = (List.toArray [lf]) ++ (List.toArray lf_tail) := by grind
+    have Htail_wf: FactoryWF (lf_tail.toArray) := by
+      rw [Hl] at newF_wf
+      apply FactoryWF.mk
+      · have newF_wf_name_nodup := newF_wf.name_nodup
+        grind
+      · intro lf
+        have newF_wf_lfuncs_wf := newF_wf.lfuncs_wf lf
+        intro Hmem
+        apply newF_wf_lfuncs_wf
+        apply Array.mem_append_right
+        assumption
+    have Hhead_wf: LFuncWF lf := by
+      rw [Hl] at newF_wf
+      have Hwf := newF_wf.lfuncs_wf
+      apply Hwf
+      apply Array.mem_append_left
+      grind
+    intro F'
+    simp only [List.foldlM]
+    unfold bind
+    unfold Except.instMonad
+    simp only []
+    unfold Except.bind
+    intro H
+    split at H
+    · contradiction
+    · rename_i F_interm HaddFacFun
+      have HF_interm_wf: FactoryWF F_interm := by
+        apply (Factory.addFactoryFunc_wf F F_wf lf) <;> assumption
+      simp only [] at H
+      apply tail_ih F_interm HF_interm_wf (lf_tail.toArray) <;> grind
+
+end Lambda
